@prefix dso: 	<https://www.w3id.org/dso#> .
@prefix dct:     	<http://purl.org/dc/terms/> .
@prefix xsd:     	<http://www.w3.org/2001/XMLSchema#> .
@prefix rdfs:    	<http://www.w3.org/2000/01/rdf-schema#> .
@prefix owl:	<http://www.w3.org/2002/07/owl#> .
@prefix foaf:    	<http://xmlns.com/foaf/0.1/> .
@prefix dbpedia-owl: 	<http://dbpedia.org/ontology/> .
@prefix rdf: 	<http://www.w3.org/1999/02/22-rdf-syntax-ns#> .
@prefix dcat:	<http://www.w3.org/ns/dcat> .
@prefix skos: <http://www.w3.org/2008/05/skos#> . 
@prefix oa:   <http://www.w3.org/ns/oa#>  .
@prefix duv:  <http://www.w3.org/ns/duv#> .

dso:	
	a 	owl:Ontology ;
	rdfs:label	"Demand and Supply Ontology (dso)"^^xsd:string ;
	rdfs:comment 	"The Demand and Supply Ontology (so) is a lightweight, extensible core vocabulary for representing existing datasets, their uses, and demands for new datasets." ;
	dct:creator	 	[foaf:name "Judie Attard"], [ foaf:name "Fabrizio Orlandi"] ; 
	dct:modified 	"2016-03-04"^^xsd:date .

#Dataset class
dso:content
	a rdf:Property, owl:ObjectProperty ;
	rdfs:label "content"^^xsd:string ;
	rdfs:comment "This property indicates the nature of the data content in a dataset." ;
	rdfs:domain	dcat:Dataset ;
	rdfs:range 	xsd:string .

#Data request class
dso:DataRequest
	a rdfs:Class, owl:Class ;
	rdfs:comment "A DataRequest class represents all the information about a newly requested dataset." ;
	rdfs:label "DataRequest"^^xsd:string .
	
dso:secondedBy
	a rdf:Property, owl:ObjectProperty ;
	rdfs:label "secondedBy"^^xsd:string ;
	rdfs:comment "This property indicates any Agent who support an existing Data Request." ;
	rdfs:domain	dso:DataRequest ;
	rdfs:range 	foaf:Agent .

dso:motivation
	a rdf:Property, owl:ObjectProperty ;
	rdfs:label "motivation"^^xsd:string ;
	rdfs:comment "This property indicates the motivation for a request for a new dataset from an Agent." ;
	rdfs:domain	dso:DataRequest ;
	rdfs:range 	xsd:string .
		
dso:keyword
	a rdf:Property, owl:ObjectProperty ;
		rdfs:subPropertyOf dcat:keyword ;
	rdfs:label "keyword"^^xsd:string ;
	rdfs:comment "This property indicates keywords that are relevant to describe the data required in a request for a new dataset from an Agent." ;
	rdfs:domain	dso:DataRequest ;
	rdfs:range 	xsd:string .
	
dso:description
	a rdf:Property, owl:ObjectProperty ;
		rdfs:subPropertyOf dct:description ;
	rdfs:label "description"^^xsd:string ;
	rdfs:comment "This property provides a description of the data required in a request for a new dataset from an Agent." ;
	rdfs:domain	dso:DataRequest ;
	rdfs:range 	xsd:string .
					
dso:license
	a rdf:Property, owl:ObjectProperty ;
		rdfs:subPropertyOf dct:license ;
	rdfs:label "license"^^xsd:string ;
	rdfs:comment "This property indicates the license of the data required in a request for a new dataset from an Agent." ;
	rdfs:domain	dso:DataRequest ;
	rdfs:range 	dct:LicenseDocument .	
	
dso:temporalRange
	a rdf:Property, owl:ObjectProperty ;
		rdfs:subPropertyOf dct:temporal ;
	rdfs:label "temporalRange"^^xsd:string ;
	rdfs:comment "This property indicates the temporal range of the data required in a request for a new dataset from an Agent." ;
	rdfs:domain	dso:DataRequest ;
	rdfs:range 	dct:PeriodOfTime .
		
dso:spatialRange
	a rdf:Property, owl:ObjectProperty ;
		rdfs:subPropertyOf dct:spatial ;
	rdfs:label "spatialRange"^^xsd:string ;
	rdfs:comment "This property indicates the spatial range of the data required in a request for a new dataset from an Agent." ;
	rdfs:domain	dso:DataRequest ;
	rdfs:range 	dct:Location .	
	
dso:requestContent
	a rdf:Property, owl:ObjectProperty ;
	rdfs:label "requestContent"^^xsd:string ;
	rdfs:comment "This property indicates the nature of the data content in a dataset request." ;
	rdfs:domain	dso:DataRequest ;
	rdfs:range 	skos:Concept .
	
dso:NatureOfContent
	a rdfs:Class, owl:Class ;
		rdfs:subClassOf skos:Concept, [
			rdf:type owl:Restriction ;
	  	owl:onProperty dso:content ;
	   	owl:allValuesFrom dso:ContentScheme
			], [
			rdf:type owl:Restriction ;
	  	owl:onProperty dso:requestContent ;
	   	owl:allValuesFrom dso:ContentScheme
			]; 
	rdfs:comment "This Class indicates the content within a Dataset (or a request for a Dataset), e.g. images, text" ;
	rdfs:label "NatureOfContent"^^xsd:string .
			
dso:language
	a rdf:Property, owl:ObjectProperty ;
		rdfs:subPropertyOf dct:language ;
	rdfs:label "language"^^xsd:string ;
	rdfs:comment "This property indicates the language of the data required in a request for a new dataset from an Agent." ;
	rdfs:domain	dso:DataRequest ;
	rdfs:range 	dct:LinguisticSystem .
	
dso:theme
	a rdf:Property, owl:ObjectProperty ;
		rdfs:subPropertyOf dcat:theme ;
	rdfs:label "theme"^^xsd:string ;
	rdfs:comment "This property indicates the themes that are relevant to describe the data required in a request for a new dataset from an Agent." ;
	rdfs:domain	dso:DataRequest ;
	rdfs:range 	skos:Concept .	
	
dso:mediaType
	a rdf:Property, owl:ObjectProperty ;
		rdfs:subPropertyOf dcat:mediaType ;
	rdfs:label "mediaType"^^xsd:string ;
	rdfs:comment "This property indicates the format of the requested Dataset." ;
	rdfs:domain	dso:DataRequest ;
	rdfs:range 	dct:MediaTypeorExtent .	
	
dso:submitter
	a rdf:Property, owl:ObjectProperty ;
	rdfs:label "request"^^xsd:string ;
	rdfs:comment "This property indicates the Agent who/which requested a new dataset." ;
	rdfs:domain	dso:DataRequest ;
	rdfs:range foaf:Agent .	

#use case class
dso:UseCase
	a rdfs:Class, owl:Class ;
	rdfs:comment "A UseCase is an example of re-use of a Distribution" ;
	rdfs:label "UseCase"^^xsd:string .

dso:usesDataset
	a rdf:Property, owl:ObjectProperty ;
	rdfs:label "usesDataset"^^xsd:string ;
	rdfs:comment "This property indicates the Dataset used in a Use case." ;
	rdfs:domain	dso:UseCase ;
	rdfs:range dcat:Dataset .
	
dso:usesDistribution
	a rdf:Property, owl:ObjectProperty ;
	rdfs:label "usesDistribution"^^xsd:string ;
	rdfs:comment "This property indicates the Distribution of a Dataset used in a Use case." ;
	rdfs:domain	dso:UseCase ;
	rdfs:range dcat:Distribution .


dso:useCaseMotivation
	a rdf:Property, owl:ObjectProperty ;
	rdfs:label "useCaseMotivation"^^xsd:string ;
	rdfs:comment "This property indicates the motivation for a UseCase." ;
	rdfs:domain	dso:DataRequest ;
	rdfs:range 	xsd:string .

dso:useCaseDescription
	a rdf:Property, owl:ObjectProperty ;
		rdfs:subPropertyOf dct:description ;
	rdfs:label "useCaseDescription"^^xsd:string ;
	rdfs:comment "This property provides a description of a UseCase." ;
	rdfs:domain	dso:UseCase ;
	rdfs:range 	xsd:string .
	
dso:useCaseURL
	a rdf:Property, owl:ObjectProperty ;
	rdfs:label "useCaseURL"^^xsd:string ;
	rdfs:comment "This property indicates the URL of a UseCase." ;
	rdfs:domain	dso:DataRequest ;
	rdfs:range 	xsd:string .
	
dso:generator
	a rdf:Property, owl:ObjectProperty ;
	rdfs:label "generator"^^xsd:string ;
	rdfs:comment "This property indicates the Agent who/which generated a new use case." ;
	rdfs:domain	dso:UseCase ;
	rdfs:range dso:Consumer .

#Distribution class
	
dso:consumer
	a rdf:Property, owl:ObjectProperty ;
	rdfs:label "consumer"^^xsd:string ;
	rdfs:comment "This property indicates the Consumer of a dataset distribution." ;
	rdfs:domain	dcat:Distribution ;
	rdfs:range 	dso:Consumer .

dso:Consumer
	a rdfs:Class, owl:Class;
		rdfs:subClassof foaf:Agent ;
	rdfs:comment "A Consumer is an entity (machine/human) who re-used a dataset distribution in a specific usecase." ;
	rdfs:label "Consumer"^^xsd:string .

dso:distributor
	a rdf:Property, owl:ObjectProperty ;
	rdfs:label "distributor"^^xsd:string ;
	rdfs:comment "This property indicates the Distributor of a dataset distribution." ;
	rdfs:domain	dcat:Distribution ;
	rdfs:range 	dso:Author .
	
dso:Distributor
	a rdfs:Class, owl:Class ;
		rdfs:subClassOf foaf:Agent ;
	rdfs:comment "A Distributor is an entity (machine/human) who is responsible for the creation of a dataset distribution." ;
	rdfs:label "Distributor"^^xsd:string .

	
dso:ContentScheme
	a skos:ConceptScheme ;
	dct:title "Reference list of nature of data content"@en .

dso:Images
	a skos:Concept ;
	skos:prefLabel "Images"@en ;
	skos:inScheme dso:ContentScheme .
	
dso:Text
	a skos:Concept ;
	skos:prefLabel "Text"@en ;
	skos:inScheme dso:ContentScheme .

dso:Numeric
	a skos:Concept ;
	skos:prefLabel "Numeric"@en ;
	skos:inScheme dso:ContentScheme .

dso:Documents
	a skos:Concept ;
	skos:prefLabel "Documents"@en ;
	skos:inScheme dso:ContentScheme .
	
dso:Applications
	a skos:Concept ;
	skos:prefLabel "Applications"@en ;
	skos:inScheme dso:ContentScheme .











